cleanup: stop relying on label injectivity (#66)

src/lib/state/DY.Lib.State.PrivateKeys.fst
@@ -46,13 +46,22 @@ instance map_types_private_keys: map_types private_key_key private_key_value = {
   ps_value_t = ps_private_key_value;
 }
 
+type long_term_key_usage_data = {
+  who: principal;
+}
+
+%splice [ps_long_term_key_usage_data] (gen_parser (`long_term_key_usage_data))
+
+instance parseable_serializeable_bytes_long_term_key_usage_data: parseable_serializeable bytes long_term_key_usage_data =
+  mk_parseable_serializeable ps_long_term_key_usage_data
+
 val long_term_key_type_to_usage:
-  long_term_key_type ->
+  long_term_key_type -> principal ->
   usage
-let long_term_key_type_to_usage sk_type =
+let long_term_key_type_to_usage sk_type who =
   match sk_type with
-  | LongTermPkEncKey usg -> PkKey usg empty
-  | LongTermSigKey usg -> SigKey usg empty
+  | LongTermPkEncKey usg -> PkKey usg (serialize _ {who})
+  | LongTermSigKey usg -> SigKey usg (serialize _ {who})
 
 val is_private_key_for:
   {|crypto_invariants|} -> trace ->
@@ -60,10 +69,10 @@ val is_private_key_for:
 let is_private_key_for #cinvs tr sk sk_type who =
   match sk_type with
   | LongTermPkEncKey usg -> (
-    is_decryption_key (long_term_key_type_to_usage sk_type) (principal_label who) tr sk
+    is_decryption_key (long_term_key_type_to_usage sk_type who) (principal_label who) tr sk
   )
   | LongTermSigKey usg -> (
-    is_signature_key (long_term_key_type_to_usage sk_type) (principal_label who) tr sk
+    is_signature_key (long_term_key_type_to_usage sk_type who) (principal_label who) tr sk
   )
 
 val is_public_key_for:
@@ -72,10 +81,10 @@ val is_public_key_for:
 let is_public_key_for #cinvs tr pk pk_type who =
   match pk_type with
   | LongTermPkEncKey usg -> (
-    is_encryption_key (long_term_key_type_to_usage pk_type) (principal_label who) tr pk
+    is_encryption_key (long_term_key_type_to_usage pk_type who) (principal_label who) tr pk
   )
   | LongTermSigKey usg -> (
-    is_verification_key (long_term_key_type_to_usage pk_type) (principal_label who) tr pk
+    is_verification_key (long_term_key_type_to_usage pk_type who) (principal_label who) tr pk
   )
 
 // The `#_` at the end is a workaround for FStarLang/FStar#3286
@@ -104,7 +113,7 @@ let initialize_private_keys = initialize_map private_key_key private_key_value #
 [@@ "opaque_to_smt"]
 val generate_private_key: principal -> state_id -> long_term_key_type -> traceful (option unit)
 let generate_private_key prin sess_id sk_type =
-  let* sk = mk_rand (long_term_key_type_to_usage sk_type) (principal_label prin) 64 in //TODO
+  let* sk = mk_rand (long_term_key_type_to_usage sk_type prin) (principal_label prin) 64 in //TODO
   add_key_value prin sess_id ({ty = sk_type}) ({private_key = sk;})
 
 [@@ "opaque_to_smt"]
